ExpressionVerifier.v
@@ -17,40 +17,57 @@ Require Import VCC.AssertionSemantics.
 Import Expressions.
 
 (*An expressions is defined*)
-Fixpoint assert_expr_defined (ex:expr): assertion:=
+Fixpoint assert_expr_eval (ex:expr)(x:ident): assertion:=
   (match ex with
-    Econst_int v ty => Atrue
-  | Etempvar id ty => Adefined id
+    Econst_int v ty => Agvariable x (Vint v)
+  | Etempvar id ty => Adefined id x
   | Ederef ex' ty =>
-    let p:= fresh_var empty in
+    let p:= fresh_var (singleton x) in
     let ty':= type_of_expr ex' in
-    Agexists p ((GEtempvar p ty')== ex' /\ Aalloc p)
+    Agexists p ((GEtempvar p ty')== ex' /\ Aalloc p x)
   | Ebinop op ex1 ex2 ty =>
-    assert_expr_defined ex1 /\
-    assert_expr_defined ex2 /\
-    Atrue (* Need type correctness?? *)
+    let x1:= fresh_var (union (free_vars_expr ex) (singleton x)) in
+    let x2:= fresh_var (union (union (free_vars_expr ex) (singleton x1)) (singleton x)) in
+    Agexists x1
+    (Agexists x2
+    (assert_expr_eval ex1 x1 /\
+    assert_expr_eval ex2 x2 /\
+    Abinop op (type_of_expr ex1) x1 x2 x )) (* Need type correctness?? *)
    end /\
    Aexpr_type ex (type_of_expr ex) 
   )%assert.
 
-Fixpoint assert_gexpr_defined (ex:gexpr): assertion:=
+Definition assert_expr_defined (ex:expr): assertion :=
+  let x := fresh_var empty in
+  Agexists x (assert_expr_eval ex x).
+
+Fixpoint assert_gexpr_eval (ex:gexpr)(x:ident): assertion:=
   match ex with
-  | Rexpr ex' => assert_expr_defined ex'
+  | Rexpr ex' => assert_expr_eval ex' x
   | GEconst_ptr p ty' =>
-    let xp:= fresh_var empty in
-    (Agexists xp ((Etempvar xp ty')== ex) /\ Aalloc xp)%assert 
-  | GEconst_nat _  _=> Atrue
-  | GEconst_bool _ _ => Atrue
-  | GEtempvar id _ => Agdefined id
+    ( Agvariable x (Vptr p))%assert 
+  | GEconst_nat n  _=> 
+    ( Agvariable x (GVnat n))%assert 
+  | GEconst_bool b _ => 
+    ( Agvariable x (GVbool b))%assert 
+  | GEtempvar id _ => Agdefined id x
   | GEderef ex' _ => 
-    let xp:= fresh_var (free_vars_expr ex' ) in
+    let xp:= fresh_var (union (free_vars_expr ex')(singleton x) ) in
     let ty':= type_of_gexpr ex' in
-    (Agexists xp ((GEtempvar xp ty')== ex' /\ Aalloc xp))%assert
+    (Agexists xp ((GEtempvar xp ty')== ex' /\ Aalloc xp x))%assert
   | GEbinop op ex1 ex2 ty =>
-    assert_gexpr_defined ex1 /\
-    assert_gexpr_defined ex2 /\
-    Atrue (* Need type correctness?? *)
+    let x1:= fresh_var (union (free_vars_expr ex) (singleton x)) in
+    let x2:= fresh_var (union (union (free_vars_expr ex) (singleton x1)) (singleton x)) in
+    Agexists x1
+    (Agexists x2
+    ( assert_gexpr_eval ex1 x1 /\
+    assert_gexpr_eval ex2 x2 /\
+    Abinop op (type_of_gexpr ex1) x1 x2 x )) 
   end.
+
+Definition assert_gexpr_defined (ex:gexpr): assertion :=
+  let x := fresh_var (free_vars_expr ex) in
+  Agexists x (assert_gexpr_eval ex x).
 
 Fixpoint assert_lvalue_defined (ex:expr): assertion:=
   match ex with
@@ -64,57 +81,153 @@ Fixpoint assert_lvalue_defined (ex:expr): assertion:=
   end.
 
 (* Correctness the previous three functions*)
+Lemma assert_expr_eval_safe:
+  forall (ex : expr) ghe (e : env) (h : heap) (id:ident),
+    [e, h, ghe]|= (assert_expr_eval ex id) ->
+    exists v, eval_expr ex e h v /\
+         find ghe id = Some (RV v).
+Proof.
+  induction ex; try solve[do 2 econstructor];
+    intros ? ? ? ? [].
+  - (*Econst_int*)
+    simpl in H. 
+    eexists; econstructor; eauto.
+    econstructor.
+  - destruct H.
+      destruct (find e id) eqn:HH; [|contradict H1; reflexivity].
+      eexists; split; eauto.
+      econstructor; eauto.
+  - destruct H as (v1 & (v2 & ?  &?) & (adr & ? & ? & ?)). 
+    destruct (h adr) eqn:HH; [|contradiction H4; reflexivity].
+    eexists; split; [econstructor;
+      econstructor; try eassumption|].
+    + fold_eval_expr.
+      simpl_env_gexpr.
+      remember (fresh_var empty) as p.
+      remember (eval_gexpr ex e h ghe v2) as HH0.
+      destruct_eval_gexpr.
+      subst HH0.
+      destruct_eval_expr.
+      simpl_find.
+      eapply eval_gexpr_expr; eauto.
+    + simpl_find.
+      simpl in H3; rewrite H3.
+      symmetry; apply gso.
+      intros ?.
+      eapply (fresh_var_spec (singleton id)).
+      apply singleton_spec; assumption.
+    
+  - (* binop *)
+    destruct H as (v1  & v2 & H1 & H2 & ?).
+    remember (fresh_var (union (free_vars_expr (Ebinop bo ex1 ex2 ty)) (singleton id)))as x1.
+    remember (fresh_var
+                  (union (union (free_vars_expr (Ebinop bo ex1 ex2 ty)) (singleton x1))
+                     (singleton id))) as x2.
+    eapply IHex1 in H1.
+    eapply IHex2 in H2.
+    destruct H1 as (v1' & H1 & ?).
+    destruct H2 as (v2' & H2 & ?).
+    destruct H as (v1'' & v2'' & v3'' & ? & ? & ? & ? ).
+    simpl_find.
+    simpl in H7.
+    destruct v3'' as [v3''|?]; try solve[inversion H7].
+    2: destruct (eval_binop h (type_of_expr ex1)  bo v1' v2'); simpl in H7; inversion H7.
+    exists v3''. split.
+    + econstructor; eauto.
+      destruct ((eval_binop h (type_of_expr ex1) bo v1' v2')) eqn:HH; inversion H7; subst.
+      auto.
+    + subst. simpl_find.
+      rewrite <- H6.
+      symmetry; repeat rewrite gso; auto.
+Qed.
+
 Lemma expr_defined_safe:
   forall (ex : expr) ghe (e : env) (h : heap),
     [e, h, ghe]|= (assert_expr_defined ex) ->
     exists v, eval_expr ex e h v.
 Proof.
+  intros. 
+  destruct H.
+  apply assert_expr_eval_safe in H.
+  destruct H as (?&?&?).
+  eexists; eauto.
+Qed.
+      
+Lemma assert_gexpr_eval_safe:
+  forall (ex : gexpr) ghe (e : env) (h : heap) (x:ident),
+    [e, h, ghe]|= (assert_gexpr_eval ex x) ->
+    exists v, eval_gexpr ex e h ghe v /\
+         find ghe x = Some v.
+Proof.
   induction ex; try solve[do 2 econstructor];
-    intros ? ? ? [].
-  - simpl in H;
-      destruct (find e id) eqn:HH; [|contradict H; reflexivity].
+    intros ? ? ? ? H.
+  - eapply assert_expr_eval_safe in H as (?&?&?).
+    do 2 econstructor; eauto.
+    econstructor; assumption.
+  - (*GEconst_ptr*)
+    do 2 econstructor.
+    eauto; constructor.
+    simpl in H; auto.
+  - (*GEconst_nat*) 
+    do 2 econstructor.
+    eauto; constructor.
+    simpl in H; auto.
+  - (*GEconst_bool*) 
+    do 2 econstructor.
+    eauto; constructor.
+    simpl in H; auto.
+  - destruct H.
+    destruct (find ghe id) eqn:HH; [|contradict H0; reflexivity].
     eexists; econstructor; eauto.
-  - destruct H as (v1 &( v2 & ? & ?) & adr & ? & ?).
+    econstructor; eauto.
+  - destruct H as (v1 &( v2 & ? & ?) & adr & ? & ? & ?).
     destruct (h adr) eqn:HH; [|contradiction H3; reflexivity].
     eexists; econstructor;
-      econstructor; try eassumption.
-    fold_eval_expr.
-    simpl_env_gexpr.
-    remember (fresh_var empty) as p.
-    remember (eval_gexpr ex e h ghe v2) as HH0.
-    destruct_eval_gexpr.
-    subst HH0.
-    destruct_eval_expr.
+      try (econstructor; econstructor); try eassumption.
+    + fold_eval_gexpr.
+      remember (fresh_var empty) as p.
+      simpl_env_gexpr.
+      remember (eval_gexpr ex e h ghe v2) as HH0.
+      destruct_eval_gexpr.
+      subst HH0.
+      simpl_find.
+      assumption.
+    + simpl in H2; rewrite H2.
+      symmetry. eapply gso.
+      intros ?.
+      eapply (fresh_var_spec (union (free_vars_expr ex) (singleton x))).
+      rewrite H4.
+      eapply union_spec. right; eapply singleton_spec; auto. 
+      
+  - (*binop*)
+    
+    destruct H as (v1  & v2 & H1 & H2 & ?).
+    
+    eapply IHex1 in H1.
+    eapply IHex2 in H2.
+    destruct H1 as (v1' & H1 & ?).
+    destruct H2 as (v2' & H2 & ?).
+    destruct H as (v1'' & v2'' & v3'' & ? & ? & ? & ? ).
     simpl_find.
-    eapply eval_gexpr_expr; eauto.
-  - (* binop *)
-    eexists. econstructor.
-    admit.
-Admitted.
+    simpl in H5.
+    exists v3''. split; auto.
+    subst; simpl_env_gexpr.
+      remember (fresh_var (union (free_vars_expr (GEbinop bo ex1 ex2 ty)) (singleton x)))as x1.
+      remember (fresh_var
+                  (union (union (free_vars_expr (GEbinop bo ex1 ex2 ty)) (singleton x1))
+                         (singleton x))) as x2.
+      econstructor; eauto.
+Qed.
+
 Lemma gexpr_defined_safe:
   forall (ex : gexpr) ghe (e : env) (h : heap),
     [e, h, ghe]|= (assert_gexpr_defined ex) ->
     exists v, eval_gexpr ex e h ghe v.
 Proof.
-  induction ex; try solve[do 2 econstructor];
-    intros ? ? ? H.
-  - eapply expr_defined_safe in H as (?&?).
-    do 2 econstructor; eauto.
-  - simpl in H.
-    destruct (find ghe id) eqn:HH; [|contradict H; reflexivity].
-    eexists; econstructor; eauto.
-  - destruct H as (v1 &( v2 & ? & ?) & adr & ? & ?).
-    destruct (h adr) eqn:HH; [|contradiction H2; reflexivity].
-    eexists; econstructor;
-      econstructor; try eassumption.
-    fold_eval_gexpr.
-    remember (fresh_var empty) as p.
-    simpl_env_gexpr.
-    remember (eval_gexpr ex e h ghe v2) as HH0.
-    destruct_eval_gexpr.
-    subst HH0.
-    simpl_find.
-    assumption.
-  - (*binop*)
-    admit.
-Admitted.
+  intros. 
+  destruct H.
+  apply assert_gexpr_eval_safe in H.
+  destruct H as (?&?&?).
+  eexists; eauto.
+  simpl_env_gexpr; eauto.
+Qed.
